progs/verif_sha.v
@@ -1,6 +1,6 @@
 Require Import floyd.proofauto.
 Require Import progs.sha.
-
+Require Import progs.SHA256.
 Local Open Scope logic.
 
 
@@ -59,6 +59,17 @@ Definition memset_spec :=
          local (`(eq p) retval) &&
        (`(array_at tuchar sh (fun _ => c) 0 n p)).
 
+Definition LBLOCK : Z := 16.   (* length of a block, in 32-bit integers *)
+Definition CBLOCK : Z := (LBLOCK * 4)%Z.  (* length of a block, in characters *)
+
+Goal forall c r,  typed_mapsto Tsh t_struct_SHA256state_st c r = TT.
+ intros.
+ simpl in r.
+ simpl_typed_mapsto.
+ destruct r as [r_h [r_Nl [r_Nh [r_data r_num]]]].
+ simpl.
+Abort.
+
 Definition s256state := (list int * (int * (int * (list int * int))))%type.
 Definition s256_h (s: s256state) := fst s.
 Definition s256_Nl (s: s256state) := fst (snd s).
@@ -66,41 +77,71 @@ Definition s256_Nh (s: s256state) := fst (snd (snd s)).
 Definition s256_data (s: s256state) := fst (snd (snd (snd s))).
 Definition s256_num (s: s256state) := snd (snd (snd (snd s))).
 
-Definition sha256state_ (c: val) : mpred :=
-   (EX r:_, !! (length (s256_h r) = 8%nat /\ length (s256_data r) = 16%nat) &&
-                typed_mapsto Tsh t_struct_SHA256state_st c r).
+Inductive s256abs :=  (* SHA-256 abstract state *)
+ S256abs: forall (hashed: list int)   (* words hashed, so far *)
+                         (delta: Z) (* length of "hashed" minus the recorded length in hl *)
+                         (data: list Z)  (* bytes in the partial block not yet hashed *)
+                     (range:  0 <= Zlength data < CBLOCK),
+                     s256abs.
 
-(*
-Definition arrayof_uint sh := 
-    arrayof tuint (fun (v : val) (v3 : reptype tuint) => mapsto sh tuint v (Vint v3)).
+Definition s256_relate (a: s256abs) (r: s256state) : Prop :=
+     match a with S256abs hashed delta data _ =>
+         s256_h r = process_msg init_registers hashed 
+       /\ Zlength (intlist_to_Zlist hashed) = 
+             delta + (Int.unsigned (s256_Nh r) * Int.modulus + Int.unsigned (s256_Nl r))
+       /\ data = map Int.unsigned (firstn (Z.to_nat (Int.unsigned (s256_num r))) (s256_data r))
+       /\ Zlength (s256_data r) = CBLOCK
+     end.
 
-Ltac simpl_array_of_t :=
- change (Tint I32 Unsigned noattr) with tuint;
- repeat 
- match goal with 
- | |- appcontext [arrayof tuint (fun v v3 => mapsto ?sh tuint v (Vint v3))] =>
-   change (arrayof tuint (fun (v: val) (v3: int) => mapsto sh tuint v (Vint v3))) 
-      with (arrayof_uint sh) 
- end.
-*)
+Definition sha256state_ (a: s256abs) (c: val) : mpred :=
+   EX r:s256state, 
+    !!  s256_relate a r  &&  typed_mapsto Tsh t_struct_SHA256state_st c r.
 
-Goal forall c r,  typed_mapsto Tsh t_struct_SHA256state_st c r = TT.
-intros.
- simpl in r.
- simpl_typed_mapsto.
- simpl in r.
- destruct r as [r_h [r_Nl [r_Nh [r_data r_num]]]].
- simpl.
-Abort.
+Definition data_block (contents: list Z) (v: val) :=
+  array_at tuchar Tsh (@ZnthV tuchar (map Int.repr contents)) 0 (Zlength contents) v.
+
+Lemma Zlength_process_block:
+  forall r b, Zlength (process_block r b) = 8.
+Proof.
+ intros. unfold process_block.
+Admitted.
+
+Definition process_block_abs (b: list int) (a: s256abs) : s256abs :=
+match a with
+| S256abs hashed delta data range =>
+    S256abs (hashed++b) (delta+CBLOCK) data range
+end.
 
 Definition sha256_block_data_order_spec :=
   DECLARE _sha256_block_data_order
-    WITH ctx : val, data: val, sh: share
+    WITH a: s256abs, b: list int, ctx : val, data: val, sh: share
    PRE [ _ctx OF tptr t_struct_SHA256state_st, _in OF tptr tvoid ]
-         PROP() LOCAL (`(eq ctx) (eval_id _ctx); `(eq data) (eval_id _in))
-         SEP (`(sha256state_ ctx); `(memory_block sh (Int.repr 64) data))
+         PROP(Zlength b = LBLOCK) 
+         LOCAL (`(eq ctx) (eval_id _ctx); `(eq data) (eval_id _in))
+         SEP (`(sha256state_ a ctx); `(data_block (intlist_to_Zlist b) data))
    POST [ tvoid ]
-          (`(sha256state_ ctx) * `(memory_block sh (Int.repr 64) data)).
+          (`(sha256state_ (process_block_abs b a) ctx) *
+            `(data_block (intlist_to_Zlist b) data)).
+
+Definition init_s256abs : s256abs.
+ apply (S256abs nil 0 nil).
+ simpl; split; reflexivity.
+Defined.
+
+Definition addlength_rel (n: Z) (a: s256abs) : s256abs :=
+ match a with S256abs hashed delta data range =>
+     S256abs hashed (delta-n) data range
+ end.
+                                  
+Definition SHA256_addlength_spec :=
+ DECLARE _SHA256_addlength
+ WITH len : Z, a: s256abs, c: val
+ PRE [ _c OF tptr t_struct_SHA256state_st , _len OF tuint ]
+   PROP ( ) 
+   LOCAL (`(eq len) (`Int.unsigned (`force_int (eval_id _len))); `(eq c) (eval_id _c))
+   SEP(`(sha256state_ a c))
+ POST [ tvoid ]
+   SEP(`(sha256state_ (addlength_rel len a) c)).
 
 Definition SHA256_Init_spec :=
   DECLARE _SHA256_Init
@@ -109,90 +150,112 @@ Definition SHA256_Init_spec :=
          PROP () LOCAL (`(eq c) (eval_id _c))
          SEP(`(typed_mapsto_ Tsh t_struct_SHA256state_st c))
   POST [ tvoid ] 
-         SEP(`(sha256state_ c)).
+         SEP(`(sha256state_ init_s256abs c)).
+
+Notation "'WITH'  x1 : t1 , x2 : t2 , x3 : t3 , x4 : t4 , x5 : t5 , x6 : t6 'PRE'  [ ] P 'POST' [ tz ] Q" :=
+     (mk_funspec (nil, tz) (t1*t2*t3*t4*t5*t6)
+           (fun x => match x with (((((x1,x2),x3),x4),x5),x6) => P%logic end)
+           (fun x => match x with (((((x1,x2),x3),x4),x5,x6)) => Q%logic end))
+            (at level 200, x1 at level 0, x2 at level 0, x3 at level 0, x4 at level 0, 
+              x5 at level 0, x6 at level 0, P at level 100, Q at level 100).
+
+Notation "'WITH'  x1 : t1 , x2 : t2 , x3 : t3 , x4 : t4 , x5 : t5 , x6 : t6 'PRE'  [ u , .. , v ] P 'POST' [ tz ] Q" :=
+     (mk_funspec ((cons u%formals .. (cons v%formals nil) ..), tz) (t1*t2*t3*t4*t5*t6)
+           (fun x => match x with (((((x1,x2),x3),x4),x5),x6) => P%logic end)
+           (fun x => match x with (((((x1,x2),x3),x4),x5),x6) => Q%logic end))
+            (at level 200, x1 at level 0, x2 at level 0, x3 at level 0, x4 at level 0, 
+             x5 at level 0, x6 at level 0, P at level 100, Q at level 100).
+
+Lemma zero_le_Zlength: forall A (l: list A), 0 <= Zlength l.
+Proof.
+intros. rewrite Zlength_correct. omega.
+Qed.
+
+Lemma grab_and_process_block_length:
+ forall n r firstr msg r' m',
+    Zlength msg >= Z_of_nat n ->
+    grab_and_process_block n r firstr msg  = (r',m') ->
+    Zlength r' = 8.
+Proof.
+ induction n; intros.
+ inv H0.
+ apply Zlength_process_block.
+ rewrite Zlength_correct in H.
+ apply Nat2Z.inj_ge in H.
+ destruct msg.
+ inv H.
+ simpl in H.
+ apply IHn in H0; auto.
+ rewrite Zlength_correct; apply Nat2Z.inj_ge.
+ omega.
+Qed.
+
+Inductive update_abs: forall (msg: list Z) (a a': s256abs), Prop :=
+| UA_short: forall msg hashed data range
+         (H: Zlength (data++msg) < CBLOCK),
+         update_abs msg 
+           (S256abs hashed 0 data range)
+           (S256abs hashed 0 (data++msg) (conj (zero_le_Zlength _ _) H))
+| UA_long: forall (msg newblock: list Z) (b: list int) hashed data (msg': list Z) 
+                      range range' a'',
+        newblock = firstn (Z.to_nat CBLOCK) (data++msg) ->
+        intlist_to_Zlist b = newblock ->
+        newblock ++ msg' = data ++ msg ->
+        update_abs msg' (S256abs (hashed++b) 0 nil range')   a'' ->
+        update_abs msg (S256abs hashed 0 data range) a''.
 
 Definition SHA256_Update_spec :=
   DECLARE _SHA256_Update
-   WITH c : val, d: val, len: Z, sh: share, A: mpred
+   WITH a: s256abs, data: list Z, c : val, d: val, sh: share, len : Z
    PRE [ _c OF tptr t_struct_SHA256state_st, _data_ OF tptr tvoid, _len OF tuint ]
-         PROP () LOCAL (`(eq c) (eval_id _c); `(eq d) (eval_id _data_); 
+         PROP (len <= Zlength data)
+         LOCAL (`(eq c) (eval_id _c); `(eq d) (eval_id _data_); 
                                   `(eq len) (`Int.unsigned (`force_int (eval_id _len))))
-         SEP(`(sha256state_ c); `(A && memory_block sh (Int.repr len) d))
+         SEP(`(sha256state_ a c); `(data_block data d))
   POST [ tvoid ] 
-         SEP(`(sha256state_ c); `A).
+         EX a':_, 
+          PROP (update_abs data a a') LOCAL ()
+          SEP(`(sha256state_ a' c); `(data_block data d)).
+
+Definition s256a_regs (a: s256abs) : list int :=
+ match a with S256abs hashed _ _ _  => 
+          process_msg init_registers hashed 
+ end.
+
+Definition sha_finish (a a': s256abs) :=
+ match a, a' with
+ | S256abs hashed delta data range,
+   S256abs hashed' delta' data' range' =>
+     hashed' = generate_and_pad (intlist_to_Zlist hashed ++ data) 0
+  /\ data'=nil /\ delta=0 /\ delta'=0
+ end.
+   
 
 Definition SHA256_Final_spec :=
   DECLARE _SHA256_Final
-   WITH md: val, c : val,  shmd: share, sh: share
+   WITH a: s256abs, md: val, c : val,  shmd: share, sh: share
    PRE [ _md OF tptr tuchar, _c OF tptr t_struct_SHA256state_st ]
          PROP (writable_share shmd) 
          LOCAL (`(eq md) (eval_id _md); `(eq c) (eval_id _c))
-         SEP(`(sha256state_ c); `(memory_block shmd (Int.repr 32) md))
+         SEP(`(sha256state_ a c); `(memory_block shmd (Int.repr 32) md))
   POST [ tvoid ] 
-         SEP(`(sha256state_ c); 
-                `(EX mdv:list (reptype tuchar), array_at tuchar shmd (ZnthV mdv) 0 32 md)).
+         EX a':s256abs,
+         PROP (sha_finish a a') LOCAL ()
+         SEP(`(sha256state_ a' c); `(data_block (intlist_to_Zlist (s256a_regs a')) md)).
 
 Definition SHA256_spec :=
   DECLARE _SHA256
-   WITH d: val, len: Z, sh: share*share, A: mpred, md: val
+   WITH d: val, len: Z, sh: share*share, data: list Z, md: val
    PRE [ _d OF tptr tuchar, _n OF tuint, _md OF tptr tuchar ]
-         PROP (writable_share (snd sh)) LOCAL (`(eq d) (eval_id _data_);
-                                  `(eq len) (`Int.unsigned (`force_int (eval_id _n)));
-                                  `(eq md) (eval_id _md))
-         SEP(`(A && memory_block (fst sh) (Int.repr len) d);
+         PROP (writable_share (snd sh)) 
+         LOCAL (`(eq d) (eval_id _data_);
+                     `(eq (Zlength data)) (`Int.unsigned (`force_int (eval_id _n)));
+                     `(eq md) (eval_id _md))
+         SEP(`(data_block data d);
                `(memory_block (snd sh) (Int.repr 32) md))
   POST [ tvoid ] 
-         SEP(`A;
-               `(EX mdv:list (reptype tuchar), array_at tuchar (snd sh) (ZnthV mdv) 0 32 md)).
-
-Module Alternate.
-
-Record sha256rep : Type :=  {
-  sr_h: Z -> int; sr_lh: Z; sr_data: Z -> int; sr_num: Z
-}.
-
-Definition field_offset' (t: type) (fld: ident) (p: val) : val :=
- match t with
-  | Tstruct id fList  att =>
-     match field_offset fld fList with
-     | Errors.OK delta => offset_val (Int.repr delta) p
-     | _ =>  Vundef
-     end
-  | _  => Vundef
-  end.
-
-Definition sha256state (r: sha256rep) (p: val) : mpred :=
-   array_at tuint Tsh (sr_h r) 0 8
-      (field_offset' t_struct_SHA256state_st _h p) 
- * field_mapsto Tsh t_struct_SHA256state_st _Nl p 
-                   (Vint (Int.repr (sr_lh r)))
- * field_mapsto Tsh t_struct_SHA256state_st _Nh p 
-                   (Vint (Int.repr (Zdiv (sr_lh r) Int.modulus)))
- * array_at tuint Tsh (sr_data r) 0 16
-      (field_offset' t_struct_SHA256state_st _data p) 
- * field_mapsto Tsh t_struct_SHA256state_st _num p 
-                 (Vint (Int.repr (sr_num r))).
-
-
-Definition sha256_block_data_order_spec :=
-  DECLARE _sha256_block_data_order
-    WITH ctx : val, b: val, sh: share
-   PRE [ _ctx OF tptr t_struct_SHA256state_st, _in OF tptr tvoid ]
-         PROP() LOCAL (`(eq ctx) (eval_id _ctx); `(eq b) (eval_id _in))
-         SEP (`(EX r:_, sha256state r ctx) * `(memory_block sh (Int.repr 64) b))
-   POST [ tvoid ]
-          (`(EX r:_, sha256state r ctx) * `(memory_block sh (Int.repr 64) b)).
-
-Definition SHA256_Init_spec :=
-  DECLARE _SHA256_Init
-   WITH c : val 
-   PRE [ _c OF tptr t_struct_SHA256state_st ]
-         PROP () LOCAL (`(eq c) (eval_id _c))
-         SEP(`(typed_mapsto_ Tsh t_struct_SHA256state_st c))
-  POST [ tvoid ] 
-         SEP(`(EX r:_, sha256state r c)).
-
-End Alternate.
+         SEP(`(data_block data d); 
+               `(data_block (SHA_256 data) md)).
 
 Definition Vprog : varspecs := (_K256, tarray tuint 64)::nil.
 
@@ -207,7 +270,7 @@ Definition Gprog : funspecs :=
 Definition Gtot := do_builtins (prog_defs prog) ++ Gprog.
 
 Lemma sha256state__isptr:
- forall c, sha256state_ c = !!(isptr c) && sha256state_ c.
+ forall a c, sha256state_ a c = !!(isptr c) && sha256state_ a c.
 Proof.
 intros. unfold sha256state_. normalize. apply f_equal.
 extensionality r.
@@ -245,6 +308,26 @@ go_lowerx.
 normalize.
 Qed.
 
+Fixpoint loops (s: statement) : list statement :=
+ match s with 
+  | Ssequence a b => loops a ++ loops b
+  | Sloop _ _ => [s]
+  | Sifthenelse _ a b => loops a ++ loops b
+  | _ => nil
+  end.
+
+Definition block_data_order_loop1 := 
+   nth 0 (loops (fn_body f_sha256_block_data_order)) Sskip.
+
+Definition block_data_order_loop2 := 
+   nth 0 (loops (fn_body f_sha256_block_data_order)) Sskip.
+
+Lemma Zlength_process_msg:
+  forall b, Zlength (process_msg init_registers b) = 8.
+Proof.
+ intros.
+Admitted.
+
 Lemma body_sha256_block_data_order: semax_body Vprog Gtot f_sha256_block_data_order sha256_block_data_order_spec.
 Proof.
 start_function.
@@ -260,23 +343,83 @@ name l_ _l.
 name Ki _Ki.
 name in_ _in.
 name ctx_ _ctx.
+name i_ _i.
+name data_ _data.
 unfold sha256state_.
 simpl_stackframe_of. 
 normalize. intros [r_h [r_Nl [r_Nh [r_data r_num]]]].
 repeat simpl_typed_mapsto.
 unfold fst,snd.
-rewrite field_mapsto_isptr.
 normalize.
-unfold s256_data in H0;
-simpl in H0; destruct H0.
-assert (Zlength r_h = 8) by (rewrite Zlength_correct; omega).
+unfold s256_relate in H1. destruct a.
+simpl in H1.
+unfold s256_Nh, s256_Nl, s256_data, s256_num, fst, snd in H1.
+destruct H1 as [? [? [? ?]]].
+assert (Zlength r_h = 8) by (subst r_h; apply Zlength_process_msg).
 
 forward. (* data = in; *)
 forward; [entailer! ;  omega | ]. (* a = ctx->h[0]; *)
 forward; [entailer! ;  omega | ]. (* b = ctx->h[1]; *)
 forward; [entailer! ;  omega | ]. (* c = ctx->h[2]; *)
 forward; [entailer! ;  omega | ]. (* d = ctx->h[3]; *)
+forward; [entailer! ;  omega | ]. (* e = ctx->h[4]; *)
+forward; [entailer! ;  omega | ]. (* f = ctx->h[5]; *)
+forward; [entailer! ;  omega | ]. (* g = ctx->h[6]; *)
+forward; [entailer! ;  omega | ]. (* h = ctx->h[7]; *)
+forward.  (* i = 0; *)
+normalize.
+simpl force_signed_int.
+normalize.
+rewrite <- H1.
 
+Fixpoint eval_ids (ids: list ident) : environ -> list val :=
+  match ids with
+  |  id::ids' => `cons (eval_id id) (eval_ids ids')
+  | nil => `nil
+ end.
+  
+Definition abcdefgh (r: list int)  : environ -> Prop :=
+  `(eq (map Vint r)) (eval_ids [_a,_b,_c,_d,_e,_f,_g,_h]).
+
+Lemma sha256_block_data_order_loop1_proof:
+  forall (Espec : OracleKind)
+     (b: list int) (data: val) (regs: list int),
+     Zlength b = LBLOCK ->
+     semax (initialized _i
+          (initialized _h
+           (initialized _g
+              (initialized _f
+                 (initialized _e
+                    (initialized _d
+                       (initialized _c
+                          (initialized _b
+                             (initialized _a
+                                (initialized _data
+   (func_tycontext f_sha256_block_data_order Vprog Gtot)))))))))))
+  (PROP ()
+   LOCAL (`(eq (map Vint regs)) (eval_ids [_a,_b,_c,_d,_e,_f,_g,_h]))
+   SEP ( `(array_at tuint Tsh (@ZnthV tuint K) 0 (Zlength K))
+                   (eval_expr (Evar _K256 (tarray tuint 64)));
+           `(arrayof_ (mapsto_ Tsh tuint) tuint 16) (eval_var _X (tarray tuint 16));
+           `(data_block (intlist_to_Zlist b) data)))
+  block_data_order_loop1
+  (normal_ret_assert
+    (PROP () 
+     LOCAL(`(eq (map Vint (rnd_64 regs K (rev b)))) (eval_ids [_a,_b,_c,_d,_e,_f,_g,_h]))
+     SEP ( `(array_at tuint Tsh (@ZnthV tuint K) 0 (Zlength K))
+                   (eval_expr (Evar _K256 (tarray tuint 64)));
+           `(array_at tuint Tsh (@ZnthV tuint b) 0 16) (eval_var _X (tarray tuint 16));
+           `(data_block (intlist_to_Zlist b) data))) ).
+Admitted.
+
+eapply semax_seq'; 
+  [ eapply semax_pre; 
+     [ | apply sha256_block_data_order_loop1_proof
+              with (regs:=r_h)(b:=b)(data:=data); eassumption ] 
+  | ].
+
+go_lower.
+entailer.
 (* . . . and so on *)
 
 Admitted.
@@ -286,8 +429,15 @@ Admitted.
 
 
 
-
-
+(*
+Ltac ff := 
+match goal with Delta := context [initialized ?i (@pair ?u ?v ?w ?x)] |- _ =>
+ let D := fresh "D" in
+  set (D := initialized i (@pair u v w x)) in Delta;
+  cbv delta [initialized] in D; simpl in D;
+  unfold D in *; clear D
+end.
+*)
 
 
 
